rudimentary event system model

txn-data-consistency/CCv_Eiger_Port_modified.thy
@@ -24,14 +24,20 @@ definition ep_version_init :: "'v ep_version" where
     v_ts = 0, v_gst = 0, v_is_pending = False\<rparr>"
 
 \<comment> \<open>Server State\<close>
+datatype 'v state_wtxn = Ready | Prep tstmp 'v | Commit 'v
 record 'v server =
+  wtxn_state :: "txid0 \<Rightarrow> key \<Rightarrow> 'v state_wtxn"
   clock :: tstmp
   lst :: tstmp
   pending_wtxns :: "txid0 \<rightharpoonup> tstmp"
   DS :: "'v datastore"
 
+definition DS_init :: "'v datastore" where
+  "DS_init \<equiv> (\<lambda>k. [ep_version_init])"
+
 \<comment> \<open>Client State\<close>
-datatype 'v state_txn = Idle | RtxnInProg "key set" "key \<rightharpoonup> 'v" | WtxnInProg svr_id "key \<rightharpoonup> 'v"
+datatype 'v state_txn = Idle | RtxnInProg "key set" "key \<rightharpoonup> 'v" | WtxnPrep "key \<rightharpoonup> 'v" |
+  WtxnCommit tstmp "key \<rightharpoonup> 'v"
 record 'v client =
   txn_state :: "'v state_txn"
   txn_sn :: sqn
@@ -40,12 +46,14 @@ record 'v client =
 
 \<comment> \<open>Global State\<close>
 record 'v state = 
-  svrs :: "svr_id \<Rightarrow> 'v server"
   cls :: "cl_id \<Rightarrow> 'v client"
+  svrs :: "svr_id \<Rightarrow> 'v server"
 
-\<comment> \<open>Events\<close>
+subsubsection \<open>Events\<close>
 
-datatype 'v ev = RInvoke "key set" cl_id | Read key 'v tstmp cl_id | RDone "key \<rightharpoonup> 'v" cl_id
+datatype 'v ev = RInvoke cl_id "key set" | Read cl_id key 'v | RDone cl_id "key \<rightharpoonup> 'v" |
+  WInvoke cl_id "key \<rightharpoonup> 'v" | WriteAll cl_id "key \<rightharpoonup> 'v" tstmp | WDone cl_id |
+  WPrep svr_id txid0 key 'v | WCommit svr_id txid0 key | Skip2
 
 fun at :: "'v ep_version list \<Rightarrow> tstmp \<Rightarrow> 'v ep_version" where
   "at [] ts = ep_version_init" |
@@ -60,8 +68,9 @@ fun newest_own_write :: "'v ep_version list \<Rightarrow> tstmp \<Rightarrow> cl
         Tn (Tn_cl sn cl') \<Rightarrow> (if cl' = cl then Some v else newest_own_write vl ts cl))
      else None)"
 
-definition read_invoke :: "key set \<Rightarrow> cl_id \<Rightarrow> 'v state \<Rightarrow> 'v state \<Rightarrow> bool" where
-  "read_invoke keys cl s s' \<equiv> 
+\<comment> \<open>Clint Events\<close>
+definition read_invoke :: "cl_id \<Rightarrow> key set \<Rightarrow> 'v state \<Rightarrow> 'v state \<Rightarrow> bool" where
+  "read_invoke cl keys s s' \<equiv> 
     txn_state (cls s cl) = Idle \<and>
     txn_state (cls s' cl) = RtxnInProg keys (Map.empty) \<and>
     txn_sn (cls s' cl) = txn_sn (cls s cl) \<and>
@@ -69,8 +78,8 @@ definition read_invoke :: "key set \<Rightarrow> cl_id \<Rightarrow> 'v state \<
     lst_map (cls s' cl) = lst_map (cls s cl) \<and>
     svrs s' = svrs s"
 
-definition read :: "key \<Rightarrow> 'v \<Rightarrow> cl_id \<Rightarrow> 'v state \<Rightarrow> 'v state \<Rightarrow> bool" where
-  "read k v cl s s' \<equiv> \<exists>keys vals.
+definition read :: "cl_id \<Rightarrow> key \<Rightarrow> 'v \<Rightarrow> 'v state \<Rightarrow> 'v state \<Rightarrow> bool" where
+  "read cl k v s s' \<equiv> \<exists>keys vals.
     txn_state (cls s cl) = RtxnInProg keys vals \<and> k \<in> keys \<and> vals k = None \<and>
     txn_state (cls s' cl) = RtxnInProg keys (vals (k \<mapsto> v)) \<and>
     v = (let vl = (DS (svrs s (loc k)) k); ver = at vl (gst (cls s cl)) in
@@ -81,8 +90,8 @@ definition read :: "key \<Rightarrow> 'v \<Rightarrow> cl_id \<Rightarrow> 'v st
     (\<forall>l. l \<noteq> loc k \<longrightarrow> lst_map (cls s' cl) = lst_map (cls s cl)) \<and>
     svrs s' = svrs s"
 
-definition read_done :: "(key \<rightharpoonup> 'v) \<Rightarrow> cl_id \<Rightarrow> 'v state \<Rightarrow> 'v state \<Rightarrow> bool" where
-  "read_done vals cl s s' \<equiv> \<exists>keys.
+definition read_done :: "cl_id \<Rightarrow> (key \<rightharpoonup> 'v) \<Rightarrow> 'v state \<Rightarrow> 'v state \<Rightarrow> bool" where
+  "read_done cl vals s s' \<equiv> \<exists>keys.
     txn_state (cls s cl) = RtxnInProg keys vals \<and> dom vals = keys \<and>
     txn_state (cls s' cl) = Idle \<and>
     txn_sn (cls s' cl) = Suc (txn_sn (cls s cl)) \<and>
@@ -90,17 +99,54 @@ definition read_done :: "(key \<rightharpoonup> 'v) \<Rightarrow> cl_id \<Righta
     lst_map (cls s' cl) = lst_map (cls s cl) \<and>
     svrs s' = svrs s"
 
+definition write_invoke :: "cl_id \<Rightarrow> (key \<rightharpoonup> 'v) \<Rightarrow> 'v state \<Rightarrow> 'v state \<Rightarrow> bool" where
+  "write_invoke cl kv_map s s' \<equiv> 
+    txn_state (cls s cl) = Idle \<and>
+    txn_state (cls s' cl) = WtxnPrep kv_map \<and>
+    txn_sn (cls s' cl) = txn_sn (cls s cl) \<and>
+    gst (cls s' cl) = gst (cls s cl) \<and>
+    lst_map (cls s' cl) = lst_map (cls s cl) \<and>
+    svrs s' = svrs s"
 
-definition prepare_write :: "key \<Rightarrow> 'v \<Rightarrow> sqn \<Rightarrow> cl_id \<Rightarrow> tstmp \<Rightarrow> svr_id \<Rightarrow> 'v state \<Rightarrow> 'v state \<Rightarrow> bool" where
-  "prepare_write k v sn cl gst_ts svr s s' \<equiv>
+definition write_all :: "cl_id \<Rightarrow> (key \<rightharpoonup> 'v) \<Rightarrow> tstmp \<Rightarrow> 'v state \<Rightarrow> 'v state \<Rightarrow> bool" where
+  "write_all cl kv_map commit_t s s' \<equiv>
+    txn_state (cls s cl) = WtxnPrep kv_map \<and>
+    (\<forall>k\<in>dom kv_map. \<exists>prep_t v.
+      wtxn_state (svrs s (loc k)) (Tn_cl (txn_sn (cls s cl)) cl) k = Prep prep_t v \<and> 
+      kv_map k = Some v \<and> prep_t \<le> commit_t) \<and>
+    txn_state (cls s' cl) = WtxnCommit commit_t kv_map \<and>
+    txn_sn (cls s' cl) = txn_sn (cls s cl) \<and>
+    gst (cls s' cl) = gst (cls s cl) \<and>
+    lst_map (cls s' cl) = lst_map (cls s cl) \<and>
+    svrs s' = svrs s"
+
+definition write_done :: "cl_id \<Rightarrow> 'v state \<Rightarrow> 'v state \<Rightarrow> bool" where
+  "write_done cl s s' \<equiv> \<exists>kv_map commit_t.
+    txn_state (cls s cl) = WtxnCommit commit_t kv_map \<and>
+    (\<forall>k\<in>dom kv_map. \<exists>v. wtxn_state (svrs s (loc k)) (Tn_cl (txn_sn (cls s cl)) cl) k = Commit v \<and>
+       kv_map k = Some v) \<and>
+    txn_state (cls s' cl) = Idle \<and>
+    txn_sn (cls s' cl) = Suc (txn_sn (cls s cl)) \<and>
+    gst (cls s' cl) = gst (cls s cl) \<and>
+    (\<forall>l. l \<in> loc ` (dom kv_map) \<longrightarrow> lst_map (cls s' cl) l = lst (svrs s l)) \<and>
+    (\<forall>l. l \<notin> loc ` (dom kv_map) \<longrightarrow> lst_map (cls s' cl) l = lst_map (cls s cl) l) \<and>
+    svrs s' = svrs s"
+
+\<comment> \<open>Server Events\<close>
+definition prepare_write :: "svr_id \<Rightarrow> txid0 \<Rightarrow> key \<Rightarrow> 'v \<Rightarrow> 'v state \<Rightarrow> 'v state \<Rightarrow> bool" where
+  "prepare_write svr t k v s s' \<equiv> \<exists>kv_map.
+    txn_state (cls s (get_cl_txn t)) = WtxnPrep kv_map \<and> k \<in> dom kv_map \<and> kv_map k = Some v \<and>
+    wtxn_state (svrs s svr) t k = Ready \<and>
+    wtxn_state (svrs s' svr) t k = Prep (clock (svrs s' svr)) v \<and>
+    (\<forall>t' k'. t' \<noteq> t \<or> k' \<noteq> k \<longrightarrow> wtxn_state (svrs s' svr) t' = wtxn_state (svrs s svr) t') \<and>
     loc k = svr \<and>
     clock (svrs s' svr) = Suc (clock (svrs s svr)) \<and>
     lst (svrs s' svr) = lst (svrs s svr) \<and>
-    pending_wtxns (svrs s' svr) (Tn_cl sn cl) = Some (clock (svrs s svr)) \<and>
-    (\<forall>t'. t' \<noteq> Tn_cl sn cl \<longrightarrow> pending_wtxns (svrs s' svr) t' = pending_wtxns (svrs s svr) t') \<and>
+    pending_wtxns (svrs s' svr) t = Some (clock (svrs s svr)) \<and>
+    (\<forall>t'. t' \<noteq> t \<longrightarrow> pending_wtxns (svrs s' svr) t' = pending_wtxns (svrs s svr) t') \<and>
     DS (svrs s' svr) k =
-      \<lparr>v_value = v, v_writer = Tn (Tn_cl sn cl), v_readerset = {},
-        v_ts = clock (svrs s svr), v_gst = gst_ts, v_is_pending = True\<rparr> # DS (svrs s svr) k \<and>
+      \<lparr>v_value = v, v_writer = Tn t, v_readerset = {}, v_ts = clock (svrs s svr),
+       v_gst = (gst (cls s (get_cl_txn t))), v_is_pending = True\<rparr> # DS (svrs s svr) k \<and>
     (\<forall>k'. k' \<noteq> k \<longrightarrow> DS (svrs s' svr) k' = DS (svrs s svr) k') \<and>
     cls s' = cls s"
 
@@ -111,17 +157,57 @@ fun find_and_commit :: "'v ep_version list \<Rightarrow> txid \<Rightarrow> tstm
       v \<lparr>v_ts := commit_t, v_is_pending := False\<rparr> # vl
     else v # (find_and_commit vl t commit_t))"
 
-definition commit_write :: "key \<Rightarrow> sqn \<Rightarrow> cl_id \<Rightarrow> tstmp \<Rightarrow> svr_id \<Rightarrow> 'v state \<Rightarrow> 'v state \<Rightarrow> bool" where
-  "commit_write k sn cl commit_t svr s s' \<equiv>
+definition commit_write :: "svr_id \<Rightarrow> txid0 \<Rightarrow> key \<Rightarrow> 'v state \<Rightarrow> 'v state \<Rightarrow> bool" where
+  "commit_write svr t k s s' \<equiv> \<exists>kv_map commit_t.
+    txn_state (cls s (get_cl_txn t)) = WtxnCommit commit_t kv_map \<and> k \<in> dom kv_map \<and>
+    (\<exists>prep_t v. wtxn_state (svrs s svr) t k = Prep prep_t v \<and> kv_map k = Some v \<and>
+      wtxn_state (svrs s' svr) t k = Commit v) \<and>
+    (\<forall>t' k'. t' \<noteq> t \<or> k' \<noteq> k \<longrightarrow> pending_wtxns (svrs s' svr) t' = pending_wtxns (svrs s svr) t') \<and>
     loc k = svr \<and>
     clock (svrs s' svr) = clock (svrs s svr) \<and>
     lst (svrs s' svr) =
       (if dom (pending_wtxns (svrs s' svr)) = {} then clock (svrs s svr)
        else Min (ran (pending_wtxns (svrs s' svr)))) \<and>
-    pending_wtxns (svrs s' svr) (Tn_cl sn cl) = None \<and>
-    (\<forall>t'. t' \<noteq> Tn_cl sn cl \<longrightarrow> pending_wtxns (svrs s' svr) t' = pending_wtxns (svrs s svr) t') \<and>
-    DS (svrs s' svr) k = find_and_commit (DS (svrs s svr) k) (Tn (Tn_cl sn cl)) commit_t \<and>
+    pending_wtxns (svrs s' svr) t = None \<and>
+    (\<forall>t'. t' \<noteq> t \<longrightarrow> pending_wtxns (svrs s' svr) t' = pending_wtxns (svrs s svr) t') \<and>
+    DS (svrs s' svr) k = find_and_commit (DS (svrs s svr) k) (Tn t) commit_t \<and>
     (\<forall>k'. k' \<noteq> k \<longrightarrow> DS (svrs s' svr) k' = DS (svrs s svr) k')"
 
-(*definition write_coord :: "key \<Rightarrow> 'v \<Rightarrow> cl_id \<Rightarrow> tstmp \<Rightarrow> tstmp" where
-  "write_coord k v cl ts \<equiv> "*)
+subsubsection \<open>The Event System\<close>
+
+definition state_init :: "'v state" where
+  "state_init \<equiv> \<lparr> 
+    cls = (\<lambda>cl. \<lparr> txn_state = Idle,
+                  txn_sn = 0,
+                  gst = 0,
+                  lst_map = (\<lambda>svr. 0) \<rparr>),
+    svrs = (\<lambda>svr. \<lparr> wtxn_state = (\<lambda>t k. Ready),
+                    clock = 0,
+                    lst = 0,
+                    pending_wtxns = Map.empty,
+                    DS = DS_init \<rparr>)
+  \<rparr>"
+
+fun state_trans :: "'v state \<Rightarrow> 'v ev \<Rightarrow> 'v state \<Rightarrow> bool" where
+  "state_trans s (RInvoke cl keys)        s' \<longleftrightarrow> read_invoke cl keys s s'" |
+  "state_trans s (Read cl k v)            s' \<longleftrightarrow> read cl k v s s'" |
+  "state_trans s (RDone cl kv_map)        s' \<longleftrightarrow> read_done cl kv_map s s'" |
+  "state_trans s (WInvoke cl kv_map)      s' \<longleftrightarrow> write_invoke cl kv_map s s'" |
+  "state_trans s (WriteAll cl kv_map cts) s' \<longleftrightarrow> write_all cl kv_map cts s s'" |
+  "state_trans s (WDone cl)               s' \<longleftrightarrow> write_done cl s s'" |
+  "state_trans s (WPrep svr t k v)        s' \<longleftrightarrow> prepare_write svr t k v s s'" |
+  "state_trans s (WCommit svr t k)        s' \<longleftrightarrow> commit_write svr t k s s'" |
+  "state_trans s Skip2 s' \<longleftrightarrow> s' = s"
+
+definition tps :: "('v ev, 'v state) ES" where
+  "tps \<equiv> \<lparr>
+    init = (=) state_init,
+    trans = state_trans
+  \<rparr>"
+
+lemmas tps_trans_defs = read_invoke_def read_def read_done_def write_invoke_def write_all_def
+  write_done_def prepare_write_def commit_write_def
+
+lemmas tps_defs = tps_def state_init_def
+
+lemma tps_trans [simp]: "trans tps = state_trans" by (simp add: tps_def)
